Fstar/fun/Implmenetations/Utils.fst
@@ -1,3 +1,46 @@
 module Utils
 
+
+module Map = FStar.OrdMap
+
 type addr = int
+
+val map_accum_l (#acc #a #b : Type) :
+                (acc -> a -> (acc * b))
+                -> acc
+                -> xs : list a
+                -> Tot (acc * list b)
+                      (decreases %[xs])
+let rec map_accum_l #_ #_ #_ f s = function
+  | []     -> s, []
+  | x :: xs ->
+    let s, y  = f s x in
+    let s, ys = map_accum_l f s xs in
+    s, y :: ys
+
+
+let test = map_accum_l (fun x acc -> x + acc, x) 0 [1;2;3]
+
+val list_to_map : #a   : eqtype
+                -> #b  : Type
+                -> xs  : list (a * b)
+                -> cmp : Map.cmp a
+                -> Map.ordmap a b cmp
+let list_to_map #_ #_ xs cmp =
+  List.Tot.Base.fold_right (fun (k,v) acc -> Map.update k v acc)
+                           xs
+                           Map.empty
+
+
+val typeOf (#a:Type u#a) : a -> Type u#a
+let typeOf #a _ = a
+
+val list_to_map_t : #a    : eqtype
+                  -> #b   : Type
+                  -> #cmp : Map.cmp a
+                  -> xs   : list (a * b)
+                  -> Map.ordmap a b cmp
+let list_to_map_t #a #b #cmp xs  =
+  List.Tot.Base.fold_right (fun (k,v) acc -> Map.update k v acc)
+                           xs
+                           Map.empty
